src/ListSumExample.v
@@ -148,9 +148,9 @@ Proof.
                     (initialL := (initialRiscvMachine_without_instructions l)).
   unfold Pipeline.evalH in Q.
   edestruct Q as [fuelL P]; try eassumption.
-  - change 14 with (5 + 9). rewrite Nat.pow_add_r.
-    pose proof (zero_lt_pow2 9).
-    forget (pow2 9) as x.
+  - change 14 with (8 + 6). rewrite Nat.pow_add_r.
+    pose proof (zero_lt_pow2 6).
+    forget (pow2 6) as x.
     apply lt_mul_mono; cbv; omega.
   - reflexivity.
   - match goal with
